\section{The Matrix Representation of a Linear Transformation}\label{sec:2.2}

\begin{note}
  In \cref{sec:2.2}, we embark on one of the most useful approaches to the analysis of a linear transformation on a finite-dimensional vector space:
  the representation of a linear transformation by a matrix.
  In fact, we develop a one-to-one correspondence between matrices and linear transformations that allows us to utilize properties of one to study properties of the other.
\end{note}

\begin{defn}\label{2.2.1}
  Let \(\V\) be a finite-dimensional vector space over \(\F\).
  An \textbf{ordered basis} for \(\V\) over \(\F\) is a basis for \(\V\) over \(\F\) endowed with a specific order;
  that is, an ordered basis for \(\V\) over \(\F\) is a finite sequence of linearly independent vectors in \(\V\) that generates \(\V\).
\end{defn}

\begin{defn}\label{2.2.2}
  For the vector space \(\vs{F}^n\), we call \(\set{\seq{e}{1,2,,n}}\) the \textbf{standard ordered basis} for \(\vs{F}^n\) over \(\F\).
  Similarly, for the vector space \(\ps[n]{\F}\), we call \(\set{1, x, \dots, x^n}\) the \textbf{standard ordered basis} for \(\ps[n]{\F}\) over \(\F\).
\end{defn}

\begin{defn}\label{2.2.3}
  Let \(\beta = \set{\seq{u}{1,2,,n}}\) be an ordered basis for a finite-dimensional vector space \(\V\) over \(\F\).
  For \(x \in \V\), let \(\seq{a}{1,2,,n} \in \F\) be the unique scalars such that
  \[
    x = \sum_{i = 1}^n a_i u_i.
  \]
  We define the \textbf{coordinate vector of \(x\) relative to \(\beta\)}, denoted \([x]_{\beta}\), by
  \[
    [x]_{\beta} = \begin{pmatrix}
      a_1    \\
      a_2    \\
      \vdots \\
      a_n
    \end{pmatrix}.
  \]
\end{defn}

\begin{defn}\label{2.2.4}
  Suppose that \(\V\) and \(\W\) are finite-dimensional vector spaces over \(\F\) with ordered bases \(\beta = \set{\seq{v}{1,2,,n}}\) and \(\gamma = \set{\seq{w}{1,2,,m}}\) over \(\F\), respectively.
  Let \(\T : \V \to \W\) be linear.
  Then for each \(j\), \(1 \leq j \leq n\), there exist unique scalars \(a_{i j} \in \F\), \(1 \leq i \leq m\), such that
  \[
    \T(v_j) = \sum_{i = 1}^m a_{i j} w_i \quad \text{for } 1 \leq j \leq n.
  \]
  We call the \(m \times n\) matrix \(A\) defined by \(A_{i j} = a_{i j}\) the \textbf{matrix representation of \(\T\) in the ordered bases \(\beta\) and \(\gamma\)} and write \(A = [\T]_{\beta}^{\gamma}\).
  If \(\V = \W\) and \(\beta = \gamma\), then we write \(A = [\T]_{\beta}\).
\end{defn}

\begin{note}
  Notice that the \(j\)th column of \(A\) is simply \([\T(v_j)]_{\gamma}\).
  Also observe that if \(\U : \V \to \W\) is a linear transformation such that \([\U]_{\beta}^{\gamma} = [\T]_{\beta}^{\gamma}\), then \(\U = \T\) by \cref{2.1.13}.
\end{note}

\begin{defn}\label{2.2.5}
  Let \(\T, \U : \V \to \W\) be arbitrary functions, where \(\V\) and \(\W\) are vector spaces over \(\F\), and let \(a \in \F\).
  We define \(\T + \U : \V \to \W\) by \((\T + \U)(x) = \T(x) + \U(x)\) for all \(x \in \V\), and \(a \T: \V \to \W\) by \((a \T)(x) = a \T(x)\) for all \(x \in \V\).
\end{defn}

\begin{thm}\label{2.7}
  Let \(\V\) and \(\W\) be vector spaces over a field \(\F\), and let \(\T, \U : \V \to \W\) be linear.
  \begin{enumerate}
    \item For all \(a \in \F\), \(a \T + \U\) is linear.
    \item Using the operations of addition and scalar multiplication in \cref{2.2.5}, the collection of all linear transformations from \(\V\) to \(\W\) is a vector space over \(\F\).
  \end{enumerate}
\end{thm}

\begin{proof}[\pf{2.7}(a)]
  Let \(x, y \in \V\) and \(c \in \F\).
  Then
  \begin{align*}
    (a \T + \U)(cx + y) & = a \T(cx + y) + \U(cx + y)            &  & \text{(by \cref{2.2.5})}    \\
                        & = a(\T(cx + y)) + c \U(x) + \U(y)      &  & \text{(by \cref{2.1.2}(b))} \\
                        & = a(c \T(x) + \T(y)) + c \U(x) + \U(y) &  & \text{(by \cref{2.1.2}(b))} \\
                        & = ac \T(x) + c \U(x) + a \T(y) + \U(y) &  & \text{(by \cref{1.2.1})}    \\
                        & = c (a \T + \U)(x) + (a \T + \U)(y).   &  & \text{(by \cref{2.2.5})}
  \end{align*}
  So \(a \T + \U\) is linear.
\end{proof}

\begin{proof}[\pf{2.7}(b)]
  Let \(\ls(\V, \W)\) be the set of all linear transformation from \(\V\) to \(\W\).
  First we show that \ref{vs1}--\ref{vs8} is true.
  Let \(f, g, h \in \ls(\V, \W)\) and let \(a, b \in \F\).
  Now we split into eight cases:
  \begin{description}
    \item[For \ref{vs1}:] We have
      \begin{align*}
        \forall x \in \V, (f + g)(x) & = f(x) + g(x) &  & \text{(by \cref{2.2.5})} \\
                                     & = g(x) + f(x) &  & \text{(by \ref{vs1})}    \\
                                     & = (g + f)(x)  &  & \text{(by \cref{2.2.5})}
      \end{align*}
      and thus \(f + g = g + f\).
    \item[For \ref{vs2}:] We have
      \begin{align*}
        \forall x \in \V, ((f + g) + h)(x) & = (f + g)(x) + h(x)    &  & \text{(by \cref{2.2.5})} \\
                                           & = (f(x) + g(x)) + h(x) &  & \text{(by \cref{2.2.5})} \\
                                           & = f(x) + (g(x) + h(x)) &  & \text{(by \ref{vs2})}    \\
                                           & = f(x) + (g + h)(x)    &  & \text{(by \cref{2.2.5})} \\
                                           & = (f + (g + h))(x)     &  & \text{(by \cref{2.2.5})}
      \end{align*}
      and thus \((f + g) + h = f + (g + h)\).
    \item[For \ref{vs3}:] We have
      \begin{align*}
        \forall x \in \V, (f + \zT)(x) & = f(x) + \zT(x)   &  & \text{(by \cref{2.2.5})} \\
                                       & = f(x) + \zv_{\W} &  & \text{(by \cref{2.1.9})} \\
                                       & = f(x)            &  & \text{(by \ref{vs3})}
      \end{align*}
      and thus \(f + \zT = f\).
    \item[For \ref{vs4}:] We have
      \begin{align*}
        \forall x \in \V, (f + ((-1)f))(x) & = f(x) + ((-1)f)(x) &  & \text{(by \cref{2.2.5})} \\
                                           & = f(x) + (-1)f(x)   &  & \text{(by \cref{2.2.5})} \\
                                           & = \zv_{\W}          &  & \text{(by \ref{vs4})}    \\
                                           & = \zT(x)            &  & \text{(by \cref{2.1.9})}
      \end{align*}
      and thus \(f + (-1)f = \zT\).
    \item[For \ref{vs5}:] We have
      \begin{align*}
        \forall x \in \V, (1f)(x) & = 1f(x) &  & \text{(by \cref{2.2.5})} \\
                                  & = f(x)  &  & \text{(by \ref{vs5})}
      \end{align*}
      and thus \(1f = f\).
    \item[For \ref{vs6}:] We have
      \begin{align*}
        \forall x \in \V, ((ab)f)(x) & = (ab) f(x)   &  & \text{(by \cref{2.2.5})} \\
                                     & = a (bf(x))   &  & \text{(by \ref{vs6})}    \\
                                     & = a ((bf)(x)) &  & \text{(by \cref{2.2.5})} \\
                                     & = (a (bf))(x) &  & \text{(by \cref{2.2.5})}
      \end{align*}
      and thus \((ab)f = a (bf)\).
    \item[For \ref{vs7}:] We have
      \begin{align*}
        \forall x \in \V, (a(f + g))(x) & = a((f + g)(x))     &  & \text{(by \cref{2.2.5})} \\
                                        & = a(f(x) + g(x))    &  & \text{(by \cref{2.2.5})} \\
                                        & = af(x) + ag(x)     &  & \text{(by \ref{vs7})}    \\
                                        & = (af)(x) + (ag)(x) &  & \text{(by \cref{2.2.5})} \\
                                        & = (af + ag)(x)      &  & \text{(by \cref{2.2.5})}
      \end{align*}
      and thus \(a(f + g) = af + ag\).
    \item[For \ref{vs8}:] We have
      \begin{align*}
        \forall x \in \V, ((a + b)f)(x) & = (a + b) f(x)    &  & \text{(by \cref{2.2.5})} \\
                                        & = af(x) + bf(x)   &  & \text{(by \ref{vs8})}    \\
                                        & = af(x) + (bf)(x) &  & \text{(by \cref{2.2.5})} \\
                                        & = (af + bf)(x)    &  & \text{(by \cref{2.2.5})}
      \end{align*}
      and thus \((a + b)f = af + bf\).
  \end{description}
  From the proofs above we see that \ref{vs1}--\ref{vs8} is true.

  By \cref{2.7}(a) and the proofs above we see that
  \[
    \forall \T, \U \in \ls(\V, \W), \T + \U = 1 \T + \U \in \ls(\V, \W)
  \]
  and
  \[
    \forall (c, \T) \in \F \times \ls(\V, \W), c \T = c \T + \zT \in \ls(\V, \W).
  \]
  Thus by \cref{1.2.1} \(\ls(\V, \W)\) is a vector space over \(\F\).
\end{proof}

\begin{defn}\label{2.2.6}
  Let \(\V\) and \(\W\) be vector spaces over \(\F\).
  We denote the vector space of all linear transformations from \(\V\) into \(\W\) by \(\ls(\V, \W)\).
  In the case that \(\V = \W\), we write \(\ls(\V)\) instead of \(\ls(\V, \W)\).
\end{defn}

\begin{thm}\label{2.8}
  Let \(\V\) and \(\W\) be finite-dimensional vector spaces over \(\F\) with ordered bases \(\beta\) and \(\gamma\) over \(\F\), respectively, and let \(\T, \U : \V \to \W\) be linear transformations.
  Then
  \begin{enumerate}
    \item \([\T + \U]_{\beta}^{\gamma} = [\T]_{\beta}^{\gamma} + [\U]_{\beta}^{\gamma}\) and
    \item \([a \T]_{\beta}^{\gamma} = a [\T]_{\beta}^{\gamma}\) for all scalars \(a \in \F\).
  \end{enumerate}
\end{thm}

\begin{proof}[\pf{2.8}]
  Let \(\beta = \set{\seq{v}{1,2,,n}}\) and \(\gamma = \set{\seq{w}{1,2,,m}}\).
  There exist unique scalars \(a_{i j}\) and \(b_{i j}\) (\(1 \leq i \leq m\), \(1 \leq j \leq n\)) such that
  \[
    \T(v_j) = \sum_{i = 1}^m a_{i j} w_i \quad \text{and} \quad \U(v_j) = \sum_{i = 1}^m b_{i j} w_i \quad \text{for } 1 \leq j \leq n.
  \]
  Hence
  \[
    (\T + \U)(v_j) = \sum_{i = 1}^m (a_{i j} + b_{i j}) w_i.
  \]
  Thus
  \[
    ([\T + \U]_{\beta}^{\gamma})_{i j} = a_{i j} + b_{i j} = ([\T]_{\beta}^{\gamma} + [\U]_{\beta}^{\gamma})_{i j}.
  \]
  So (a) is proved, and the proof of (b) is similar.
\end{proof}
